Start new EC theories for arrays and word arrays

eclib/JWord_array.ec
@@ -250,8 +250,178 @@ abstract theory WArray.
   op init256 (f:int -> W256.t) =
     init (fun i => f (i %/ 32) \bits8 (i%%32)).
 
+  (* ------------------------------------------------- *)
+
+  clone import PolyArray as ArrayW8.
+
+  op of_array8 (a: W8.t ArrayW8.t) = init8 (fun i -> a.[i]).
+
+  op to_array8 (a: t) = ArrayW8.init (fun i -> get8 a i).
+
+
+op (a: ArrayN' Wws): WArrayN.initWS (fun i -> a.[i])
+op (a: WArrayN'): ArrayN.init (fun i -> getWS a i)
+  
+
 end WArray.
 
+(* Array of words, where the word size is any number of bytes *)
+abstract theory ArrayWords
+    (* size of a word in bytes *)
+    op sizeW: int.
+    axiom gt0_sizeW: 0 < sizeW.
+
+    (* size of the array in words *)
+    op sizeA: int.
+    axiom gt0_sizeA: 0 < sizeA.
+
+    clone BitWord as Word with
+        op size <- 8 * sizeW
+        proof gt0_size by done.
+
+    clone PolyArray as ArrayN with
+        size <= sizeA
+        proof ge0_size by done.
+
+    (* Equivalent array of bytes *)
+    clone WArray as WArrayN with
+        size <= sizeW * sizeA
+        proof ge0_size by done.
+
+    (* Conversion between WArrayN.t and Word.t ArrayN.t *)
+    clone W_WS as Wu8 with
+        op sizeS <- W8.size, op sizeB <- Word.size, op r <- sizeW,
+        theory WS <- W8, theory WB <- Word
+        proof gt0_r by done, sizeBrS by done.
+
+    (* direct means offset in bytes, not in words *)
+    op wa_get_direct (t: WArrayN.t) (i: int): Word.t =
+        Wu8.pack'R_t (Wu8.Pack.init (fun j => t.[i+j])).
+    abbrev wa_get (t: WArrayN.t) (i: int): Word.t = wa_get_direct t (sizeW*i).
+    op wa_set_direct (t: WArrayN.t) (i: int) (w: Word.t) =
+        WArrayN.init (fun k => if i <= k < i + sizeW then w \bits8 (k-i) else t.[k]).
+
+    op of_word_array (a: Word.t ArrayN.t) =
+        WArrayN.init (fun i => a.[i %/ sizeW] \bits8 (i%%sizeW)).
+    op to_word_array (a: WArrayN.t) =
+        ArrayN.init (fun i -> wa_get a i).
+
+    op get_direct (a: Word.t ArrayN.t) = wa_get_direct (of_word_array a).
+    op set_direct (a: Word.t ArrayN.t) (i: int) (w: Word.t) =
+        to_word_array (wa_set_direct (of_word_array a) i w).
+
+end ArrayWords.
+
+(* Array slicing *)
+theory SubArray.
+    op sizeS: int.
+    axiom gt0_sizeS: 0 < sizeS.
+
+    op sizeB: int.
+    axiom gt0_sizeB: 0 < sizeB.
+
+    (* Sub-array *)
+    clone PolyArray as ArrayS with
+        size <= sizeS
+        proof ge0_size by done.
+
+    (* Base array *)
+    clone PolyArray as ArrayB with
+        size <= sizeB
+        proof ge0_size by done.
+
+  op get_sub (a: 'a ArrayB.t) (i: int) = ArrayS.init (fun j -> a.[i + j]).
+
+  op set_sub (a: 'a ArrayB.t) (i: int) (b: 'a ArrayS.t) =
+    ArrayB.init (fun j -> if i <= j < i + sizeS then b.[j - i] else a.[j]).
+end SubArray.
+
+theory SubArrayDirect.
+    op sizeW: int.
+    axiom gt0_sizeW: 0 < sizeW.
+
+    op sizeS: int.
+    axiom gt0_sizeS: 0 < sizeS.
+
+    op sizeB: int.
+    axiom gt0_sizeB: 0 < sizeB.
+
+    clone BitWord as Word with
+        op size <- 8 * sizeW
+        proof gt0_size by done.
+
+    clone ArrayWords as ArrayWordsS with
+        op sizeW <- sizeW, op sizeA <- sizeS, theory Word <- Word
+        proof gt0_sizeW by done, gt0_sizeA by done.
+
+    clone ArrayWords as ArrayWordsB with
+        op sizeW <- sizeW, op sizeA <- sizeB, theory Word <- Word
+        proof gt0_sizeW by done, gt0_sizeA by done.
+
+    op get_sub_direct (a: Word.t ArrayWordsB.ArrayN.t) (i: int) =
+        ArrayWordsS.ArrayN.init (fun j -> ArrayWordsB.get_direct a (i + j)).
+
+    op set_sub_direct (a: W16.t ArrayB.t) (i: int) (b: W16.t ArrayS.t) =
+        let aw = ArrayWordsB.of_word_array a in
+        let bw = ArrayWordsS.of_word_array b in
+        (* FIXME: change init8 and get8 to init and _.[_] *)
+        ArrayWordsB.to_word_array (
+            ArrayWordsB.WArrayN.init8 (fun j ->
+            if i <= j < i * sizeW * sizeS then get8 bw (j - i) else get8 aw j
+            )
+        ).
+end SubArrayDirect.
+
+(*
+theory ArrayWords16.
+  op size: int.
+  clone PolyArray as ArrayN with size <= size.
+  clone WArray as WArrayN with size <= 2 * size.
+  (* FIXME: prove axioms of cloned theories. *)
+
+  op of_w16_array (a: W16.t ArrayN.t) = WArrayN.init16 (fun i -> a.[i]).
+  op to_w16_array (a: WArrayN.t) = ArrayN.init (fun i -> get16 a i).
+
+  op get16_direct (a: W16.t ArrayN.t) = WArrayN.get16_direct (of_w16_array a).
+  op set16_direct (a: W16.t ArrayN.t) (i: int) (w: W16.t) =
+    to_w16_array (WArrayN.set16_direct (of_w16_array a) i w).
+
+end ArrayWords16.
+
+theory SubArray16Direct.
+  op sizeS: int.
+  op sizeB: int.
+
+  clone ArrayWords16 as ArrayWords16S with size <= sizeS.
+  clone ArrayWords16 as ArrayWords16B with size <= sizeB.
+
+  op get_sub_direct (a: W16.t ArrayB.t) (i: int) =
+    ArrayWords16S.ArrayN.init (fun j -> get16_direct (ArrayWords16B.of_w16_array a) (i + j)).
+
+
+  op set_sub_direct (a: W16.t ArrayB.t) (i: int) (b: W16.t ArrayS.t) =
+    let aw = ArrayWords16B.of_w16_array a in
+    let bw = ArrayWords16S.of_w16_array b in
+    (* FIXME: change init8 and get8 to init and _.[_] *)
+      ArrayWords16B.to_w16_array (
+        ArrayWords16B.WArrayN.init8 (fun j ->
+          if i <= j < i * 2 * sizeS then get8 bw (j - i) else get8 aw j
+        )
+      ).
+
+end SubArray16Direct.
+*)
+
+(* TODO: do this for pairs of Wsizes. Do this as generic theory. exemple: JWord.ec, theory W_WS and clones. *)
+
+
+(*
+from Jasmin require import JWord_array.
+require import Array8.
+
+clone export WArray as WArray8  with op size <- 8.
+clone export ArrayWords8 as ArrayWords8_8 with op size <- 8, theory ArrayN <- Array8, theory WArrayN <- WArray8.
+*)
 
 
  
